lax aes256gcm without testing

crypto_hst/symmetric/AEAD.AES256_GCM.fst
@@ -9,38 +9,34 @@ open Hacl.SBuffer
 open Symmetric.AES
 open GCM
 
+module U32 = FStar.UInt32
+
 #set-options "--lax"
 
 (* Block cipher function AES256 *)
 
-private val aes256: key:u8s{length key = 32} ->
-    input:u8s{length input = 16 /\ disjoint key input} ->
-    out:u8s{length out = 16 /\ disjoint key out /\ disjoint input out} ->
-    STL unit
-    (requires (fun h -> live h key /\ live h input /\ live h out))
-    (ensures (fun h0 r h1 -> live h1 key /\ live h1 input /\ live h1 out))	   
+private val aes256: key:u8s{length key = 32} -> input:u8s{length input = 16} ->
+    out:u8s{length out = 16} -> Stl unit
+
 let aes256 key input out =
+  push_frame();
   let w = create (uint8_to_sint8 0uy) 240ul in
   let sbox = create (uint8_to_sint8 0uy) 256ul in
   let inv_sbox = create (uint8_to_sint8 0uy) 256ul in
   mk_sbox sbox;
   mk_inv_sbox inv_sbox;
   keyExpansion key w sbox;
-  cipher out input w sbox
+  cipher out input w sbox;
+  pop_frame()
 
 (* Main AEAD functions *)
-val aead_encrypt: plaintext:u8s ->
-    tag:u8s{length tag = 16 /\ disjoint plaintext tag} ->
-    key:u8s{length tag = 32 /\ disjoint plaintext key /\ disjoint tag key} ->
-    nonce:u8s{length nonce = 12 /\ disjoint plaintext nonce /\ disjoint tag nonce /\ disjoint key nonce} ->
-    ciphertext:u8s{length ciphertext = length plaintext /\ disjoint plaintext ciphertext /\ disjoint tag ciphertext /\ disjoint key ciphertext /\ disjoint nonce ciphertext} ->
-    clen:nat{length ciphertext = clen} ->
-    ad:u8s{disjoint plaintext ad /\ disjoint tag ad /\ disjoint key ad /\ disjoint nonce ad /\ disjoint ciphertext ad} ->
-    adlen:nat{length ad = adlen} ->
-    STL unit
-    (requires (fun h -> live h plaintext /\ live h tag /\ live h key /\ live h nonce /\ live h ciphertext /\ live h ad))
-    (ensures (fun h0 r h1 -> live h1 plaintext /\ live h1 tag /\ live h1 key /\ live h1 nonce /\ live h1 ciphertext /\ live h1 ad))
-let aead_encrypt plaintext tag key nonce ciphertext clen ad adlen =
-    GCM.encrypt #32 aes256 key nonce ad adlen plaintext ciphertext clen tag
+val aead_encrypt: ciphertext:u8s -> tag:u8s{length tag = 16} ->
+    key:u8s{length key = 32} -> nonce:u8s{length nonce = 12} ->
+    plaintext:u8s{length plaintext = length ciphertext} ->
+    len:u32{length ciphertext = U32.v len} ->
+    ad:u8s -> adlen:u32{length ad = U32.v adlen} ->
+    Stl unit
+let aead_encrypt ciphertext tag key nonce plaintext len ad adlen =
+    GCM.encrypt #32 aes256 ciphertext tag key nonce ad adlen plaintext len
 
 (* TODO: AEAD decrypt function *)
